WIP adapting `touchObject`, `getObject` & its variants for new ASpec TA
Signed-off-by: Robert Sison <robert.sison@unimelb.edu.au>

proof/refine/RISCV64/KHeap_R.thy
@@ -15,12 +15,284 @@ lemma lookupAround2_known1:
 
 context begin interpretation Arch . (*FIXME: arch_split*)
 
+(* From Invariants_AI of main experimental-timeprot branch. -robs *)
+term in_ta
+term obj_in_ta
+thm obj_in_ta_def2
+
+definition
+  obj_in_ta2 :: "obj_ref \<Rightarrow> 'z::state_ext state \<Rightarrow> bool"
+where
+  "obj_in_ta2 ref s \<equiv> \<exists>ko. f_kheap True s ref = Some ko"
+
+definition
+  obj_in_ta2' :: "obj_ref \<Rightarrow> kernel_state \<Rightarrow> bool"
+where
+  "obj_in_ta2' ref s \<equiv> \<exists>ko. ksPSpace s ref = Some ko"
+
+lemma
+  "obj_in_ta ref s \<Longrightarrow> obj_in_ta2 ref s"
+  unfolding obj_in_ta_def2 obj_in_ta2_def obj_at_def
+  by (clarsimp simp:obind_def ta_filter_def)
+
+(* New for ExecSpec level. XXX: The ASpec version of this was retired by Scott,
+   so I'm trialling adapting its replacement to the ExecSpec level below. -robs
+abbreviation ta_obj_upd' :: "machine_word \<Rightarrow> Structures_H.kernel_object \<Rightarrow> machine_state \<Rightarrow> machine_state"
+  where
+  "ta_obj_upd' p ko ms \<equiv> machine_state.touched_addresses_update ((\<union>) (obj_range' p ko)) ms"
+*)
+
+(* New and experimental: To correspond with touch_object. -robs *)
+thm touch_object_def2
+definition touchObject :: "machine_word \<Rightarrow> unit kernel" where
+  "touchObject ptr \<equiv> do
+     kh <- gets ksPSpace;
+     assert (kh ptr \<noteq> None);
+     obj <- return $ the $ kh ptr;
+     doMachineOp $ addTouchedAddresses (obj_range' ptr obj)
+   od"
+
+(* New for ExecSpec level, adapted from KHeap_A. -robs *)
+
+term ms_ta_update
+(* Note: Should the naming convention have the prime `'` be at the end, or
+   is there any reason these need to end with the suffix `_update`? -robs *)
+abbreviation (input)
+  ms_ta'_update :: "(machine_word set \<Rightarrow> machine_word set) \<Rightarrow>
+    kernel_state \<Rightarrow> kernel_state" where
+ "ms_ta'_update f \<equiv> \<lambda>s. ksMachineState_update (machine_state.touched_addresses_update f) s"
+
+abbreviation ms_ta'_obj_update :: "machine_word \<Rightarrow> kernel_object \<Rightarrow> kernel_state \<Rightarrow> kernel_state"
+  where
+  "ms_ta'_obj_update p ko s \<equiv> ms_ta'_update ((\<union>) (obj_range' p ko)) s"
+
+lemma simpler_doMachineOp_getTouchedAddresses_def:
+  "doMachineOp getTouchedAddresses \<equiv> gets (\<lambda>s. machine_state.touched_addresses $ ksMachineState s)"
+  by (clarsimp simp: bind_def doMachineOp_def getTouchedAddresses_def simpler_gets_def
+                        simpler_modify_def select_f_def return_def)
+
+lemma ksMachineState_update_normalise [simp]:
+  "s\<lparr>ksMachineState := f (ksMachineState s)\<rparr> = ksMachineState_update f s"
+  by simp
+
+lemma simpler_doMachineOp_addTouchedAddresses_def:
+  "doMachineOp (addTouchedAddresses S) \<equiv> modify (ms_ta'_update ((\<union>) S))"
+  by (clarsimp simp: doMachineOp_def bind_def addTouchedAddresses_def simpler_gets_def
+                     simpler_modify_def select_f_def return_def)
+
+lemma dmo_addTouchedAddresses_wp':
+  "\<lbrace>\<lambda>s. Q () (ms_ta'_update (\<lambda>ta. S \<union> ta) s)\<rbrace> doMachineOp (addTouchedAddresses S) \<lbrace>Q\<rbrace>"
+  apply (simp add: simpler_doMachineOp_addTouchedAddresses_def)
+  by (wp select_f_wp)
+
+(* XXX: Not sure how to deal with the uncertainty of the type of `ko` here.
+   Declaring its type as below doesn't seem to work... -robs
+term ko_at
+term ko_at'
+lemma touchObj_wp:
+  "\<lbrace>\<lambda>s. \<forall>ko. (ko_at'::(Structures_H.kernel_object \<Rightarrow> obj_ref \<Rightarrow> kernel_state \<Rightarrow> bool))
+      (ko::Structures_H.kernel_object) p s \<longrightarrow> Q () (ms_ta'_obj_update p ko s) \<rbrace>
+   touchObject p \<lbrace>Q\<rbrace>"
+  apply (wpsimp simp:touch_object_def2 wp: dmo_addTouchedAddresses_wp)
+  apply (clarsimp simp:obj_at_def)
+  done
+*)
+
+lemma touchObject_wp':
+  "\<lbrace>\<lambda>s. Q () (ms_ta'_obj_update p (the (ksPSpace s p)) s) \<rbrace>
+   touchObject p \<lbrace>Q\<rbrace>"
+  apply(wpsimp simp:touchObject_def wp:dmo_addTouchedAddresses_wp')
+  done
+
+thm touch_object_wp touch_object_wp'
+term ko_at
+term "ko_at'"
+term \<top>
+thm obj_at_def
+
+lemma touchObject_corres_others:
+  "corres (=) (obj_at (\<lambda>ko. (\<not> is_CNode ko) \<and>
+       (case ko of ArchObj ao \<Rightarrow> \<not> is_PageTable ao \<and> \<not> is_DataPage ao | _ \<Rightarrow> True)) ptr)
+     (obj_at' \<top> ptr) (touch_object ptr) (touchObject ptr)"
+  apply(simp add: touchObject_def touch_object_def2)
+  apply(rule corres_split')
+     apply(rule corres_stronger_no_failI)
+      apply(rule no_fail_pre, wp)
+      apply(rule TrueI)
+     apply(clarsimp simp:simpler_gets_def)
+     apply(rename_tac s s')
+     apply(rule_tac x="(kheap s, s)" in bexI)
+      apply simp (* XXX: Dummy out r as \<top>\<top> *)
+      (* XXX: This version fills in r as pspace_relation, but we don't seem to need it this early.
+      apply(clarsimp simp:state_relation_def split:prod.splits)
+      apply assumption *)
+     apply(force simp:simpler_gets_def)
+    apply clarsimp
+    apply(rule corres_split')
+       apply(rule corres_underlyingI)
+        apply(clarsimp simp:in_assert)
+        apply(rename_tac kh kh' s s' ko)
+        apply(rule_tac x="((), s)" in bexI)
+         apply(clarsimp split:prod.splits)
+         apply simp (* XXX: Dummy out r as \<top>\<top> *)
+        (* XXX: Is there a better way to pass these through than forcing ?Q and ?Q'? *)
+        apply(subgoal_tac "obj_at (\<lambda>ko. (\<not> is_CNode ko) \<and>
+          (case ko of ArchObj ao \<Rightarrow> \<not> is_PageTable ao \<and> \<not> is_DataPage ao | _ \<Rightarrow> True)) ptr s \<and>
+          kh = kheap s")
+         prefer 2
+         apply assumption
+        apply(subgoal_tac "obj_at' (\<lambda>_. True) ptr s' \<and> kh' = ksPSpace s'")
+         prefer 2
+         apply assumption
+        apply(clarsimp simp:in_assert return_def obj_at_def)
+       apply(clarsimp simp:in_assert return_def obj_at'_def)
+      prefer 4
+      apply(wpsimp simp:obj_at_def return_def)
+     prefer 4
+     apply(wpsimp simp:obj_at'_def return_def)
+     apply blast
+    apply clarsimp
+    (* XXX: Ah wait. Do we need something relating the range of the two objects? *)
+    apply(rule corres_underlyingI)
+     apply clarsimp
+     apply(clarsimp simp:simpler_doMachineOp_addTouchedAddresses_def simpler_modify_def
+       simpler_do_machine_op_addTouchedAddresses_def)
+     apply(clarsimp simp:state_relation_def pspace_relation_def)
+     apply(rule conjI)
+      apply(clarsimp simp:cdt_relation_def)
+     apply(clarsimp simp:obj_range_def obj_range'_def)
+     apply(rename_tac kh kh' s s')
+(*
+     apply(subgoal_tac "touched_addresses (ksMachineState s') \<subseteq> touched_addresses (machine_state s)")
+      prefer 2
+      apply(clarsimp simp:machine_state_relation_def)
+*)
+     apply(clarsimp simp:machine_state_relation_def)
+     (* XXX: Again, is there a better way to pass these through than forcing ?Q and ?Q'? *)
+     apply(subgoal_tac "obj_at (\<lambda>ko. (\<not> is_CNode ko) \<and>
+       (case ko of ArchObj ao \<Rightarrow> \<not> is_PageTable ao \<and> \<not> is_DataPage ao | _ \<Rightarrow> True)) ptr s \<and>
+       kh = kheap s")
+      prefer 2
+      apply assumption
+     apply(subgoal_tac "obj_at' (\<lambda>_. True) ptr s' \<and> kh' = ksPSpace s'")
+      prefer 2
+      apply assumption
+     prefer 3
+     apply wpsimp
+    prefer 3
+    apply wpsimp
+    apply blast
+   prefer 2
+   apply(clarsimp simp:simpler_doMachineOp_addTouchedAddresses_def simpler_modify_def)
+  (* FIXME: We need something in pspace_relation that relates the address footprint of the
+     kheap object `ko` with that of the ksPSpace object `kh' ptr`. *)
+  (* FIXME: Also, this demand that the kheap and ksPSpace object at `ptr` occupy exactly the same
+     addresses is probably too strong. Hadn't we reasoned that refinement could make the TA set
+     smaller, due to choosing to touch only a subset of the TA overapproximated by the ASpec? *)
+  apply(rule conjI)
+   prefer 2
+   apply(force simp:machine_state_relation_def)
+  (* Trying this first. *)
+  apply(subgoal_tac "mask_range ptr (objBitsKO (the (kh' ptr))) \<subseteq> obj_addrs (the (kh ptr)) ptr")
+   apply blast
+  (* Should the `pspace_relation` relate the two objects at `ptr`? *)
+  apply(erule_tac x=ptr in ballE)
+   prefer 2
+   apply(force simp:obj_at_def)
+  apply clarsimp
+  apply(clarsimp simp:other_obj_relation_def objBitsKO_def mask_def)
+  apply(case_tac "the (kheap s ptr)")
+      defer
+      (* Case: TCB *)
+      apply(clarsimp simp:other_obj_relation_def objBitsKO_def tcbBlockSizeBits_def mask_def split:kernel_object.splits)
+      apply(force intro:eq_refl)
+     (* Case: Endpoint *)
+     apply(clarsimp simp:other_obj_relation_def objBitsKO_def epSizeBits_def mask_def split:kernel_object.splits)
+     apply(force intro:eq_refl)
+    (* Case: Notification *)
+    apply(clarsimp simp:other_obj_relation_def objBitsKO_def ntfnSizeBits_def mask_def split:kernel_object.splits)
+    apply(force intro:eq_refl)
+   (* Case: ArchObj *)
+   apply(clarsimp simp:other_obj_relation_def objBitsKO_def)
+   apply(rename_tac s s' aobj)
+   apply(case_tac aobj)
+     (* Case: ASIDPool *)
+     apply(clarsimp simp:other_obj_relation_def objBitsKO_def)
+     apply(clarsimp split:kernel_object.splits arch_kernel_object.splits)
+     apply(clarsimp simp:pageBits_def archObjSize_def mask_def)
+     apply(force intro:eq_refl)
+    (* Case: PageTable *)
+    apply(force simp:obj_at_def) (* XXX: Excluding PageTable for now
+    apply(clarsimp simp:other_obj_relation_def objBitsKO_def)
+    apply(clarsimp simp:pte_relation_def)
+    apply(erule_tac x="0" in allE)
+    apply clarsimp
+    (* XXX: Not sure if this would be a good use of the relaxation of pspace_relation
+       to allow TA to shrink... even if I could prove it. *)
+    apply(clarsimp simp:archObjSize_def pte_bits_def table_size_def ptTranslationBits_def word_size_bits_def)
+    apply(rule word_leI)
+    defer
+    *)
+   (* Case: DataPage *)
+   apply(force simp:obj_at_def) (* XXX: Excluding DataPage for now
+   apply(clarsimp simp:other_obj_relation_def objBitsKO_def)
+(*
+   apply(clarsimp simp:pspace_dom_def obj_relation_cuts_def2)
+*)
+   apply(rename_tac dev sz)
+   apply(erule_tac x="ptr + (1 << pageBits)" in allE)
+   apply(erule_tac x="(\<lambda>_ obj. obj = (if dev then KOUserDataDevice else KOUserData))" in allE)
+   apply clarsimp
+   apply(erule impE)
+    apply(clarsimp simp:pageBits_def)
+    (* XXX: No dice here either.
+    apply(clarsimp simp:pageBitsForSize_def split:vmpage_size.splits)
+    apply(rule conjI)
+     apply clarsimp
+     apply(clarsimp simp:pageBits_def pageBitsForSize_def) *)
+    apply(rule_tac x="1" in exI)
+    apply(rule conjI)
+     apply(clarsimp simp:pageBits_def pageBitsForSize_def)
+    apply(clarsimp simp:pageBitsForSize_def split:vmpage_size.splits)
+    apply(clarsimp simp:pageBits_def ptTranslationBits_def)
+    (* XXX: Nope. *)
+    defer
+   defer
+   *)
+  (* Case: CNode *)
+  apply(force simp:obj_at_def)
+  (* XXX: Excluding CNode for now. FIXME: Prove.
+  apply(clarsimp simp:obj_relation_cuts_def2)
+  apply(clarsimp simp:cte_map_def cap_relation_def well_formed_cnode_n_def cte_relation_def split:kernel_object.splits arch_kernel_object.splits if_splits)
+  *)
+  done
+
+thm get_object_def
+term f_kheap
+
+(* XXX: Adaptations to ExecSpec -robs *)
+definition
+  ta_filter' :: "bool \<Rightarrow> machine_word set \<Rightarrow> kernel_object \<Rightarrow> obj_ref \<Rightarrow> kernel_object option" where
+  "ta_filter' apply ta obj ptr \<equiv> if ~apply \<or> obj_range' ptr obj \<subseteq> ta then Some obj else None"
+
+abbreviation f_ksPSpace :: "bool \<Rightarrow> kernel_state \<Rightarrow> obj_ref \<Rightarrow> kernel_object option" where
+  "f_ksPSpace apply s \<equiv> ksPSpace s |>> ta_filter' apply (touched_addresses (ksMachineState s))"
+
+(* Copied from PSpaceFuns_H for experimentation. To correspond with get_object. -robs *)
+definition getObject_x_copy where
+"getObject_x_copy ta_f ptr\<equiv> (do
+        map \<leftarrow> gets $ psMap \<circ> ksPSpace;
+        (before, after) \<leftarrow> return ( lookupAround2 (fromPPtr ptr) map);
+        (ptr', val) \<leftarrow> maybeToMonad before;
+        loadObject (fromPPtr ptr) ptr' after val
+od)"
+
 lemma obj_at_getObject:
   assumes R:
   "\<And>a b n ko s obj::'a::pspace_storable.
   \<lbrakk> (a, b) \<in> fst (loadObject t t n ko s); projectKO_opt ko = Some obj \<rbrakk> \<Longrightarrow> a = obj"
-  shows "\<lbrace>obj_at' P t\<rbrace> getObject t \<lbrace>\<lambda>(rv::'a::pspace_storable) s. P rv\<rbrace>"
-  by (auto simp: getObject_def obj_at'_def in_monad valid_def
+  shows "\<lbrace>obj_at' P t\<rbrace> getObject_x_copy ta_f t \<lbrace>\<lambda>(rv::'a::pspace_storable) s. P rv\<rbrace>"
+  by (auto simp: getObject_x_copy_def obj_at'_def in_monad valid_def
                  split_def lookupAround2_known1
            dest: R)
 
@@ -36,10 +308,10 @@ lemma loadObject_default_inv:
 
 lemma getObject_inv:
   assumes x: "\<And>p q n ko. \<lbrace>P\<rbrace> loadObject p q n ko \<lbrace>\<lambda>(rv :: 'a :: pspace_storable). P\<rbrace>"
-  shows      "\<lbrace>P\<rbrace> getObject p \<lbrace>\<lambda>(rv :: 'a :: pspace_storable). P\<rbrace>"
-  by (simp add: getObject_def split_def | wp x)+
+  shows      "\<lbrace>P\<rbrace> getObject_x_copy ta_f p \<lbrace>\<lambda>(rv :: 'a :: pspace_storable). P\<rbrace>"
+  by (simp add: getObject_x_copy_def split_def | wp x)+
 
-lemma getObject_inv_tcb [wp]: "\<lbrace>P\<rbrace> getObject l \<lbrace>\<lambda>(rv :: Structures_H.tcb). P\<rbrace>"
+lemma getObject_inv_tcb [wp]: "\<lbrace>P\<rbrace> getObject_x_copy ta_f l \<lbrace>\<lambda>(rv :: Structures_H.tcb). P\<rbrace>"
   apply (rule getObject_inv)
   apply simp
   apply (rule loadObject_default_inv)
@@ -68,8 +340,8 @@ lemma no_fail_loadObject_default [wp]:
   done
 
 lemma no_fail_getObject_tcb [wp]:
-  "no_fail (tcb_at' t) (getObject t :: tcb kernel)"
-  apply (simp add: getObject_def split_def)
+  "no_fail (tcb_at' t) (getObject_x_copy ta_f t :: tcb kernel)"
+  apply (simp add: getObject_x_copy_def split_def)
   apply (rule no_fail_pre)
    apply wp
   apply (clarsimp simp add: obj_at'_def objBits_simps'
@@ -98,16 +370,14 @@ lemmas page_table_at_obj_at'
 
 
 lemma corres_get_tcb:
-  (* FIXME: But surely we will need a correspondence with get_Tcb True quite soon;
-     therefore we'll need to adapt getObject accordingly. -robs *)
-  "corres (tcb_relation \<circ> the) (tcb_at t) (tcb_at' t) (gets (get_tcb False t)) (getObject t)"
+  "corres (tcb_relation \<circ> the) (tcb_at t and obj_in_ta2 t) (tcb_at' t) (gets (get_tcb ta_f t)) (getObject_x_copy ta_f t)"
   apply (rule corres_no_failI)
    apply wp
   apply (clarsimp simp add: gets_def get_def return_def bind_def get_tcb_def)
   apply (frule in_inv_by_hoareD [OF getObject_inv_tcb])
   apply (clarsimp simp add: obj_at_def is_tcb obj_at'_def projectKO_def
                             projectKO_opt_tcb split_def
-                            getObject_def loadObject_default_def in_monad)
+                            getObject_x_copy_def loadObject_default_def in_monad)
   apply (case_tac koa)
    apply (simp_all add: fail_def return_def)
   apply (case_tac bb)
@@ -116,8 +386,8 @@ lemma corres_get_tcb:
   apply (drule bspec)
    apply clarsimp
    apply blast
-  apply (clarsimp simp add: other_obj_relation_def
-                            lookupAround2_known1)
+  apply (clarsimp simp add: other_obj_relation_def obj_in_ta2_def obind_def ta_filter_def
+                            lookupAround2_known1 split: if_splits)
   done
 
 lemma lookupAround2_same1[simp]:
@@ -128,8 +398,8 @@ lemma lookupAround2_same1[simp]:
   done
 
 lemma getObject_tcb_at':
-  "\<lbrace> \<top> \<rbrace> getObject t \<lbrace>\<lambda>r::tcb. tcb_at' t\<rbrace>"
-  by (clarsimp simp: valid_def getObject_def in_monad
+  "\<lbrace> \<top> \<rbrace> getObject_x_copy ta_f t \<lbrace>\<lambda>r::tcb. tcb_at' t\<rbrace>"
+  by (clarsimp simp: valid_def getObject_x_copy_def in_monad
                      loadObject_default_def obj_at'_def split_def
                      in_magnitude_check objBits_simps')
 
@@ -387,8 +657,8 @@ lemma getObject_obj_at':
   assumes x: "\<And>q n ko. loadObject p q n ko =
                 (loadObject_default p q n ko :: ('a :: pspace_storable) kernel)"
   assumes P: "\<And>(v::'a::pspace_storable). (1 :: machine_word) < 2 ^ (objBits v)"
-  shows      "\<lbrace> \<top> \<rbrace> getObject p \<lbrace>\<lambda>r::'a::pspace_storable. obj_at' ((=) r) p\<rbrace>"
-  by (clarsimp simp: valid_def getObject_def in_monad
+  shows      "\<lbrace> \<top> \<rbrace> getObject_x_copy ta_f p \<lbrace>\<lambda>r::'a::pspace_storable. obj_at' ((=) r) p\<rbrace>"
+  by (clarsimp simp: valid_def getObject_x_copy_def in_monad
                      loadObject_default_def obj_at'_def
                      split_def in_magnitude_check lookupAround2_char1
                      x P project_inject objBits_def[symmetric])
@@ -397,7 +667,7 @@ lemma getObject_valid_obj:
   assumes x: "\<And>p q n ko. loadObject p q n ko =
                 (loadObject_default p q n ko :: ('a :: pspace_storable) kernel)"
   assumes P: "\<And>(v::'a::pspace_storable). (1 :: machine_word) < 2 ^ (objBits v)"
-  shows "\<lbrace> valid_objs' \<rbrace> getObject p \<lbrace>\<lambda>rv::'a::pspace_storable. valid_obj' (injectKO rv) \<rbrace>"
+  shows "\<lbrace> valid_objs' \<rbrace> getObject_x_copy ta_f p \<lbrace>\<lambda>rv::'a::pspace_storable. valid_obj' (injectKO rv) \<rbrace>"
   apply (rule hoare_chain)
     apply (rule hoare_vcg_conj_lift)
      apply (rule getObject_obj_at' [OF x P])
@@ -416,8 +686,8 @@ lemma typeError_inv [wp]:
   "\<lbrace>P\<rbrace> typeError x y \<lbrace>\<lambda>rv. P\<rbrace>"
   by (simp add: typeError_def|wp)+
 
-lemma getObject_cte_inv [wp]: "\<lbrace>P\<rbrace> (getObject addr :: cte kernel) \<lbrace>\<lambda>rv. P\<rbrace>"
-  apply (simp add: getObject_def loadObject_cte split_def)
+lemma getObject_cte_inv [wp]: "\<lbrace>P\<rbrace> (getObject_x_copy ta_f addr :: cte kernel) \<lbrace>\<lambda>rv. P\<rbrace>"
+  apply (simp add: getObject_x_copy_def loadObject_cte split_def)
   apply (clarsimp simp: valid_def in_monad)
   apply (clarsimp simp: typeError_def in_monad magnitudeCheck_def
                  split: kernel_object.split_asm if_split_asm option.split_asm)
@@ -427,15 +697,15 @@ lemma getObject_ko_at:
   assumes x: "\<And>q n ko. loadObject p q n ko =
                 (loadObject_default p q n ko :: ('a :: pspace_storable) kernel)"
   assumes P: "\<And>(v::'a::pspace_storable). (1 :: machine_word) < 2 ^ (objBits v)"
-  shows      "\<lbrace> \<top> \<rbrace> getObject p \<lbrace>\<lambda>r::'a::pspace_storable. ko_at' r p\<rbrace>"
+  shows      "\<lbrace> \<top> \<rbrace> getObject_x_copy ta_f p \<lbrace>\<lambda>r::'a::pspace_storable. ko_at' r p\<rbrace>"
   by (subst eq_commute, rule getObject_obj_at' [OF x P])
 
 lemma getObject_ko_at_tcb [wp]:
-  "\<lbrace>\<top>\<rbrace> getObject p \<lbrace>\<lambda>rv::tcb. ko_at' rv p\<rbrace>"
+  "\<lbrace>\<top>\<rbrace> getObject_x_copy ta_f p \<lbrace>\<lambda>rv::tcb. ko_at' rv p\<rbrace>"
   by (rule getObject_ko_at | simp add: objBits_simps')+
 
 lemma OMG_getObject_tcb:
-  "\<lbrace>obj_at' P t\<rbrace> getObject t \<lbrace>\<lambda>(tcb :: tcb) s. P tcb\<rbrace>"
+  "\<lbrace>obj_at' P t\<rbrace> getObject_x_copy ta_f t \<lbrace>\<lambda>(tcb :: tcb) s. P tcb\<rbrace>"
   apply (rule obj_at_getObject)
   apply (clarsimp simp: loadObject_default_def in_monad)
   done
@@ -447,26 +717,33 @@ lemma setObject_nosch:
   apply (wp x | simp)+
   done
 
-lemma getObject_ep_inv: "\<lbrace>P\<rbrace> (getObject addr :: endpoint kernel) \<lbrace>\<lambda>rv. P\<rbrace>"
+lemma getObject_ep_inv: "\<lbrace>P\<rbrace> (getObject_x_copy ta_f addr :: endpoint kernel) \<lbrace>\<lambda>rv. P\<rbrace>"
   apply (rule getObject_inv)
   apply (simp add: loadObject_default_inv)
   done
 
 lemma getObject_ntfn_inv:
-  "\<lbrace>P\<rbrace> (getObject addr :: Structures_H.notification kernel) \<lbrace>\<lambda>rv. P\<rbrace>"
+  "\<lbrace>P\<rbrace> (getObject_x_copy ta_f addr :: Structures_H.notification kernel) \<lbrace>\<lambda>rv. P\<rbrace>"
   apply (rule getObject_inv)
   apply (simp add: loadObject_default_inv)
   done
 
-lemma get_ep_inv'[wp]: "\<lbrace>P\<rbrace> getEndpoint ep \<lbrace>\<lambda>rv. P\<rbrace>"
-  by (simp add: getEndpoint_def getObject_ep_inv)
+(* Copied from Endpoint_H to ensure they point to the experimental getObject copy. -robs *)
+definition getEndpoint_x_copy :: "bool \<Rightarrow> 64 word \<Rightarrow> endpoint kernel" where
+  "getEndpoint_x_copy \<equiv> getObject_x_copy"
 
-lemma get_ntfn_inv'[wp]: "\<lbrace>P\<rbrace> getNotification ntfn \<lbrace>\<lambda>rv. P\<rbrace>"
-  by (simp add: getNotification_def getObject_ntfn_inv)
+definition getNotification_x_copy :: "bool \<Rightarrow> 64 word \<Rightarrow> notification kernel" where
+  "getNotification_x_copy \<equiv> getObject_x_copy"
+
+lemma get_ep_inv'[wp]: "\<lbrace>P\<rbrace> getEndpoint_x_copy ta_f ep \<lbrace>\<lambda>rv. P\<rbrace>"
+  by (simp add: getEndpoint_x_copy_def getObject_ep_inv)
+
+lemma get_ntfn_inv'[wp]: "\<lbrace>P\<rbrace> getNotification_x_copy ta_f ntfn \<lbrace>\<lambda>rv. P\<rbrace>"
+  by (simp add: getNotification_x_copy_def getObject_ntfn_inv)
 
 lemma get_ep'_valid_ep[wp]:
-  "\<lbrace> invs' and ep_at' ep \<rbrace> getEndpoint ep \<lbrace> valid_ep' \<rbrace>"
-  apply (simp add: getEndpoint_def)
+  "\<lbrace> invs' and ep_at' ep \<rbrace> getEndpoint_x_copy ta_f ep \<lbrace> valid_ep' \<rbrace>"
+  apply (simp add: getEndpoint_x_copy_def)
   apply (rule hoare_chain)
   apply (rule getObject_valid_obj)
      apply simp
@@ -476,8 +753,8 @@ lemma get_ep'_valid_ep[wp]:
   done
 
 lemma get_ntfn'_valid_ntfn[wp]:
-  "\<lbrace> invs' and ntfn_at' ep \<rbrace> getNotification ep \<lbrace> valid_ntfn' \<rbrace>"
-  apply (simp add: getNotification_def)
+  "\<lbrace> invs' and ntfn_at' ep \<rbrace> getNotification_x_copy ta_f ep \<lbrace> valid_ntfn' \<rbrace>"
+  apply (simp add: getNotification_x_copy_def)
   apply (rule hoare_chain)
   apply (rule getObject_valid_obj)
      apply simp
@@ -534,7 +811,7 @@ lemma set_ep_distinct' [wp]:
   "\<lbrace>pspace_distinct'\<rbrace> setEndpoint ep v  \<lbrace>\<lambda>rv. pspace_distinct'\<rbrace>"
   unfolding setEndpoint_def by wp
 
-crunches setEndpoint, getEndpoint
+crunches setEndpoint, getEndpoint_x_copy
   for pspace_canonical'[wp]: "pspace_canonical'"
   and pspace_in_kernel_mappings'[wp]: "pspace_in_kernel_mappings'"
 
@@ -554,8 +831,8 @@ lemma setEndpoint_pred_tcb_at'[wp]:
   done
 
 lemma get_ntfn_ko':
-  "\<lbrace>\<top>\<rbrace> getNotification ep \<lbrace>\<lambda>rv. ko_at' rv ep\<rbrace>"
-  apply (simp add: getNotification_def)
+  "\<lbrace>\<top>\<rbrace> getNotification_x_copy ta_f ep \<lbrace>\<lambda>rv. ko_at' rv ep\<rbrace>"
+  apply (simp add: getNotification_x_copy_def)
   apply (rule getObject_ko_at)
    apply simp
   apply (simp add: objBits_simps')
@@ -800,8 +1077,8 @@ lemma real_cte_at':
                     del: disjCI)
 
 lemma no_fail_getEndpoint [wp]:
-  "no_fail (ep_at' ptr) (getEndpoint ptr)"
-  apply (simp add: getEndpoint_def getObject_def split_def)
+  "no_fail (ep_at' ptr) (getEndpoint_x_copy True ptr)"
+  apply (simp add: getEndpoint_x_copy_def getObject_x_copy_def split_def)
   apply (rule no_fail_pre)
    apply wp
   apply (clarsimp simp add: obj_at'_def objBits_simps' lookupAround2_known1)
@@ -814,24 +1091,21 @@ lemma no_fail_getEndpoint [wp]:
   done
 
 lemma getEndpoint_corres:
-  "corres ep_relation (ep_at ptr) (ep_at' ptr)
-     (get_endpoint ptr) (getEndpoint ptr)"
+  "corres ep_relation (ep_at ptr and obj_in_ta2 ptr) (ep_at' ptr)
+     (get_endpoint ptr) (getEndpoint_x_copy True ptr)"
   apply (rule corres_no_failI)
    apply wp
-  apply (simp add: get_simple_ko_def getEndpoint_def get_object_def
-                   getObject_def bind_assoc ep_at_def2)
+  apply (simp add: get_simple_ko_def getEndpoint_x_copy_def get_object_def
+                   getObject_x_copy_def bind_assoc ep_at_def2)
   apply (clarsimp simp: in_monad split_def bind_def gets_def get_def return_def)
   apply (clarsimp simp: assert_def fail_def obj_at_def return_def is_ep partial_inv_def)
   apply (clarsimp simp: loadObject_default_def in_monad in_magnitude_check objBits_simps')
   apply (clarsimp simp add: state_relation_def pspace_relation_def)
   apply (drule bspec)
    apply blast
-  apply (simp add: other_obj_relation_def obind_def ta_filter_def)
-  apply clarsimp
-  sorry (* FIXME: broken by touched-addrs -robs
-    Well, we won't know it's in touched_addresses if the ExecSpec didn't add it.
+  apply (simp add: other_obj_relation_def)
+  apply (clarsimp simp: obj_in_ta2_def obind_def ta_filter_def split:if_splits)
   done
-*)
 
 declare magnitudeCheck_inv [wp]
 
@@ -918,6 +1192,10 @@ fun exst_same' :: "Structures_H.kernel_object \<Rightarrow> Structures_H.kernel_
 where
   "exst_same' (KOTCB tcb) (KOTCB tcb') = exst_same tcb tcb'" |
   "exst_same' _ _ = True"
+
+. (* XXX: DOWN TO HERE. Perhaps figure out how to adapt the Haskell spec itself for
+     getObject, getEndpoint and getNotification so we can do away with their `_x_copy`
+     versions before moving on to experiment with adapting setObject? -robs
 
 lemma setObject_other_corres:
   fixes ob' :: "'a :: pspace_storable"
